codelib/CodeLib.lean
@@ -2,6 +2,7 @@ import CodeLib.Attrs
 import CodeLib.Basic
 import CodeLib.Entry
 import CodeLib.Equivalence
+import CodeLib.List
 import CodeLib.UInt32
 import CodeLib.UInt64
 import CodeLib.WordCodec
